zqy_verif.v
@@ -876,3 +876,529 @@ Definition Gprog : funspecs :=
     (* insert_spec *)
     (* delete_spec *)
   ]).
+
+(***********************************************************************
+Main proofs
+***********************************************************************)
+
+Lemma Z_length_minus_1 : forall a l, Z_length (a :: l) - 1 = Z_length l.
+Proof.
+  intros.
+  unfold Z_length.
+  simpl length.
+  lia.
+Qed.
+
+Lemma Z_length_plus_1 : forall a l, (Z_length l) + 1 = Z_length (a :: l).
+Proof.
+  intros.
+  unfold Z_length.
+  simpl length.
+  lia.
+Qed.
+
+Lemma Z_length_plus : forall l1 l2, 
+  (Z_length l1) + (Z_length l2) = Z_length (l1 ++ l2).
+Proof.
+  intros.
+  unfold Z_length.
+  rewrite app_length.
+  lia.
+Qed.
+
+(* quick unfold *)
+(* TODO: maybe not useful *)
+Ltac unfold_list_rep := unfold list_rep, list_full_rep.
+
+(* proof for split_K *)
+Theorem body_split_K: 
+  semax_body Vprog Gprog f_split_K split_K_spec.
+Proof.
+  start_function.
+  forward_call.                         (* res = list_new(); *)
+  Intros vret.
+  unfold_list_rep.
+  Intros head_latter tail_latter.
+  Intros head tail.
+  unfold Z_length at 1.
+  simpl Datatypes.length.
+  simpl list_1n_rep.
+  Intros. subst.
+  apply semax_if_seq.
+  forward_if.
+  { (* k = 0 *)
+    assert (k = 0)%nat by lia.
+    subst.
+    forward.
+    forward.                            (* res->head = l->head; *)
+    forward.
+    { sep_apply (list_1n_rep_saturate_local_tail_nullval l). entailer!. }
+    forward.                            (* res->tail = l->tail; *)
+    forward.
+    forward.                            (* res->size = l->size; *)
+    forward.                            (* l->head = NULL; *)
+    forward.                            (* l->tail = NULL; *)
+    forward.                            (* l->size = 0u; *)
+    forward.                            (* return res; *)
+    Exists vret l.
+    simpl list_prefix.
+    unfold_list_rep.
+    Exists nullval nullval.
+    Exists head tail.
+    entailer!.
+    simpl list_1n_rep.
+    entailer!.
+  }
+  { 
+    forward.
+    apply semax_if_seq.
+    forward_if.                         (* if (k < l->size) *)
+    { 
+      assert (k < length l)%nat.
+      { 
+        (* TODO：这段真的复杂 *)
+        unfold Z_length in H2.
+        unfold Int.unsigned, Int.intval in H2.
+        simpl in H2.
+        rewrite Int.Z_mod_modulus_eq in H2.
+        assert (100 < Int.modulus) by rep_lia.
+        assert (Z.of_nat (Datatypes.length l) < Int.modulus) by rep_lia.
+        pose proof (Zle_0_nat (Datatypes.length l)).
+        pose proof (Zmod_small (Z.of_nat (Datatypes.length l)) (Int.modulus)).
+        rewrite Nat2Z.inj_lt.
+        rewrite <- Zmod_small with (n:=Int.modulus).
+        - exact H2.
+        - split; assumption.
+      }
+      forward_call (l, p, k, head, tail).
+                                        (* nd = move(l, k); *)
+      { 
+        unfold list_full_rep.
+        entailer!.
+      }
+      Intros res.
+      unfold list_single_out.
+      (* TODO：和下面的重复好多 *)
+      destruct (list_nth_out l k) as [[l1 z] l2] eqn:E.
+      apply list_nth_split in E.
+      destruct E as [E1 E2].
+      pose proof (list_index_some l k H3).
+      destruct H4 as [x E3].
+      rewrite E3 in E2.
+      subst.
+      unfold node_in_list.
+      Intros tail1 head2.
+      forward.
+      { sep_apply list_1n_rep_valid_pointer_tail2. entailer!. }
+      forward.                          (* res->tail = l->tail; *)
+      unfold node_rep.
+      forward.
+      { sep_apply list_1n_rep_saturate_local_tail_nullval. entailer!. }
+      forward.                          (* l->tail = nd->prev; *)
+      forward.                          (* res->head = nd; *)
+      forward.
+      destruct k; [ contradiction | ].
+      remember (list_prefix l (S k)) as l1.
+      (* show l1 <> [] *)
+      pose proof E3 as E3_copy.
+      apply list_index_prefix in E3_copy.
+      destruct l1; [ rewrite <- Heql1 in E3_copy; contradiction | ].
+      pose proof (list_cons_app l1 z).
+      destruct H4 as [l3 [a H4]].
+      destruct H4 as [H4 [H5 H6]].
+      rewrite H4.
+      sep_apply list_1n_split.
+      Intros head' tail'.
+      simpl list_1n_rep at 2.
+      Intros old_head.
+      subst old_head. subst tail1.
+      unfold node_rep.
+      forward.                          (* nd->prev->next = NULL; *)
+      forward.                          (* nd->prev = NULL; *)
+      forward.
+      forward.                          (* res->size = l->size - k; *)
+      forward.                          (* l->size = k; *)
+      forward.                          (* return res; *)
+      Exists vret (x :: l2).
+      entailer!.
+Abort.
+
+(* proof for list_new *)
+Theorem body_list_new: 
+  semax_body Vprog Gprog f_list_new list_new_spec.
+Proof.
+  start_function.
+  forward_call (sizeof t_struct_list).  (* mallocN *)
+  { computable. }
+  Intros p.
+  rewrite memory_block_data_at_ by auto.
+  forward.                              (* l->head = NULL;  *)
+  forward.                              (* l->tail = NULL;  *)
+  forward.                              (* l->size = 0;     *)
+  forward.                              (* return;          *)
+  Exists p. 
+  unfold_list_rep.
+  Exists nullval nullval.
+  simpl list_1n_rep.
+  entailer!.
+Qed.
+
+(* proof for list_free *)
+Theorem body_list_free: 
+  semax_body Vprog Gprog f_list_free list_free_spec.
+Proof.
+  start_function.
+  unfold_list_rep.
+  Intros head tail.
+  forward.                              (* tmp = l->head;   *)
+  forward_while
+  ( EX l' : list Z, EX head' : val, 
+    EX prev' : val, 
+    PROP ()
+    LOCAL (temp _l p; temp _tmp head')
+    SEP (data_at Tsh t_struct_list 
+      (Vint (Int.repr (Z_length l')), (head', tail)) p * 
+      list_1n_rep l' head' tail prev' nullval))%assert.
+  { Exists l head nullval. entailer!. }
+  { destruct l'; entailer!. }
+  { (* loop body *)
+    destruct l'.
+    { simpl. Intros. contradiction. }
+    simpl. unfold node_rep. Intros old_head.
+    forward.
+    forward.                            (* l->head = tmp->next; *) 
+    forward_call (head', sizeof t_struct_node); [solve_free | ].
+                                        (* freeN(tmp, sizeof (struct node)); *)
+    forward.
+    forward.                            (* l->size -= 1;    *)
+    forward.                            (* tmp = l->head;   *)
+    Exists (l', old_head, head').
+    entailer!.
+    rewrite Z_length_minus_1.
+    entailer!.
+  }
+  subst head'.
+  sep_apply list_head_null.
+  Intros.
+  forward_call (p, sizeof t_struct_list); [solve_free | ].
+                                        (* freeN(l, sizeof (struct list)); *)
+  subst; simpl list_1n_rep.
+  entailer!.
+Qed.
+
+(* proof for get_size *)
+Theorem body_get_size: 
+  semax_body Vprog Gprog f_get_size get_size_spec.
+Proof.
+  start_function. 
+  unfold_list_rep.
+  Intros head tail.
+  forward.
+  forward.
+  unfold_list_rep.
+  Exists head tail.
+  entailer!.
+Qed.
+
+(* proof for next *)
+Theorem body_next: 
+  semax_body Vprog Gprog f_next next_spec.
+Proof.
+  start_function.
+  unfold node_rep.
+  forward.
+  forward.                              (* return p->next; *)
+Qed.
+
+(* proof for rnext *)
+Theorem body_rnext: 
+  semax_body Vprog Gprog f_rnext rnext_spec.
+Proof.
+  start_function.
+  unfold node_rep.
+  forward.
+  { sep_apply list_1n_rep_saturate_local_tail_nullval; entailer!. }
+  forward.                              (* return p->prev; *)
+Qed.
+
+(* proof for begin *)
+Theorem body_begin: 
+  semax_body Vprog Gprog f_begin begin_spec.
+Proof.
+  start_function. 
+  unfold_list_rep.
+  Intros.
+  forward.
+  forward.                              (* return l->head; *)
+  Exists head.
+  entailer.
+  sep_apply node_in_list_begin.
+  entailer!.
+Qed.
+
+(* proof for end *)
+Theorem body_end: 
+  semax_body Vprog Gprog f_end end_spec.
+Proof.
+  start_function. 
+  unfold_list_rep.
+  Intros.
+  forward.
+  { sep_apply list_1n_rep_saturate_local_tail_nullval; entailer!. }
+  forward.                              (* return l->tail; *)
+  Exists tail.
+  entailer.
+  sep_apply node_in_list_end.
+  entailer!.
+Qed.
+
+(* proof for rbegin, the same as end *)
+Theorem body_rbegin: 
+  semax_body Vprog Gprog f_rbegin rbegin_spec.
+Proof.
+  start_function. 
+  unfold_list_rep.
+  Intros.
+  forward.
+  { sep_apply list_1n_rep_saturate_local_tail_nullval; entailer!. }
+  forward.                              (* return l->tail; *)
+  Exists tail.
+  entailer.
+  sep_apply node_in_list_end.
+  entailer!.
+Qed.
+
+(* proof for rend, the same as begin *)
+Theorem body_rend: 
+  semax_body Vprog Gprog f_rend rend_spec.
+Proof.
+  start_function. 
+  unfold_list_rep.
+  Intros.
+  forward.
+  forward.                              (* return l->head; *)
+  Exists head.
+  entailer.
+  sep_apply node_in_list_begin.
+  entailer!.
+Qed.
+
+(* proof for move *)
+Theorem body_move: 
+  semax_body Vprog Gprog f_move move_spec.
+Proof.
+  start_function.
+  unfold_list_rep.
+  Intros.
+  forward.                              (* res = l->head; *)
+  forward_loop
+  ( EX pos' : nat, 
+    EX dis : nat, 
+    EX res' : val, 
+    PROP ((0 <= pos')%nat; (pos' + dis = pos)%nat; (dis < length l)%nat)
+    LOCAL (temp _res res'; temp _l p; 
+      temp _pos (Vint (Int.repr (Z.of_nat pos'))))
+    SEP (data_at Tsh t_struct_list
+          (Vint (Int.repr (Z_length l)), (head, tail)) p;
+    list_single_out l dis head tail res'))%assert.
+  { 
+    Exists pos 0%nat head.
+    entailer!.
+    apply node_in_list_begin.
+  }
+  { 
+    entailer!.
+  }
+  {
+    unfold list_single_out.
+    assert (HE1 : pos' <> 0%nat).
+    { 
+      intro. subst. 
+      simpl in HRE.
+      lia.
+    }
+    assert (HE2 : (dis + 1 < Datatypes.length l)%nat) by lia.
+    destruct (list_nth_out l dis) as [[l1 y] l2] eqn:E.
+    pose proof E as E_copy.
+    apply list_nth_split in E.
+    destruct E as [E1 E2].
+    pose proof (list_index_some l dis H3).
+    destruct H4 as [x E3].
+    rewrite E3 in E2.
+    subst y.
+    unfold node_in_list.
+    Intros tail1 head2.
+    unfold node_rep.
+    forward.                            (* res = res->next; *)
+    forward.                            (* pos -= 1u; *)
+    Exists ((pos' - 1)%nat, (dis + 1)%nat, head2).
+    simpl fst. simpl snd.
+    entailer!; [ do 2 f_equal; lia | ].
+    unfold list_single_out.
+    (* TODO: 感觉这部分重复率挺高的 *)
+    destruct (list_nth_out l (dis + 1)) as [[l3 z] l4] eqn:E.
+    pose proof E as E_copy2.
+    apply list_nth_split in E.
+    destruct E as [E1 E2].
+    pose proof (list_index_some l (dis + 1)%nat HE2).
+    destruct H2 as [x1 E4].
+    rewrite E4 in E2.
+    subst.
+    unfold node_in_list.
+    Exists res'.
+    (* show l2 <> [] *)
+    pose proof list_nth_out_step.
+    specialize (H2 l (list_prefix l (dis + 1)) l4).
+    specialize (H2 (list_prefix l dis) l2 x1 x dis).
+    rewrite Nat.add_1_r in *.
+    specialize (H2 E_copy2 E_copy).
+    destruct H2.
+    rewrite H2, H8.
+    simpl list_1n_rep at 2.
+    Intros old_head.
+    Exists old_head.
+    entailer!.
+    eapply derives_trans; [ | apply list_1n_merge ].
+    simpl list_1n_rep.
+    Exists head2.
+    unfold node_rep.
+    entailer.
+  }
+  forward.                              (* return res; *)
+  Exists res'.
+  assert (pos' = 0%nat) by lia.
+  subst pos'.
+  simpl plus.
+  entailer!.
+Qed.
+
+(* proof for merge *)
+Theorem body_merge: 
+  semax_body Vprog Gprog f_merge merge_spec.
+Proof.
+  start_function.
+  unfold_list_rep.
+  Intros head1 tail1 head2 tail2.
+  forward.
+  forward_if                            (* if (l2->head != NULL) *)
+  (PROP (l2 <> [])
+   LOCAL (temp _l1 p1; temp _l2 p2)
+   SEP (data_at Tsh t_struct_list
+          (Vint (Int.repr (Z_length l1)), (head1, tail1)) p1;
+   list_1n_rep l1 head1 tail1 nullval nullval;
+   data_at Tsh t_struct_list
+     (Vint (Int.repr (Z_length l2)), (head2, tail2)) p2;
+   list_1n_rep l2 head2 tail2 tail1 nullval)).
+  { 
+    destruct l2; [ simpl list_1n_rep at 2; Intros; contradiction | ].
+    simpl list_1n_rep.
+    Intros old_head.
+    forward.
+    forward.
+    { sep_apply list_1n_rep_saturate_local_tail_nullval; entailer!. }
+    unfold node_rep.
+    forward.                            (* l2->head->prev = l1->tail; *)
+    entailer!.
+    { discriminate. }
+    simpl list_1n_rep.
+    Exists old_head.
+    unfold node_rep.
+    entailer!.
+  }
+  { 
+    forward_call (p2, sizeof t_struct_list); [solve_free | ].
+                                        (* freeN(l, sizeof (struct list)); *)
+    forward.                            (* return; *)
+    entailer!.
+    destruct l2; simpl list_1n_rep.
+    2: {
+      Intros old_head.
+      unfold node_rep. 
+      entailer!.
+      sfcn.
+    }
+    rewrite app_nil_r.
+    unfold_list_rep.
+    Exists head1 tail1.
+    entailer!.
+  }
+  assert_PROP (is_pointer_or_null tail1).
+  { sep_apply list_1n_rep_saturate_local_tail_nullval; entailer!. }
+  assert_PROP (is_pointer_or_null tail2).
+  {
+    pose proof (list_1n_rep_saturate_local_tail l2 head2 tail2 tail1 nullval H).
+    sep_apply H0.
+    entailer!.
+  }
+  forward.
+  apply semax_if_seq.
+  forward_if.                           (* if (l1->tail != NULL) *)
+  {
+    destruct l1; simpl list_1n_rep; 
+      [ | Intros old_head1; sep_apply list_1n_rep_valid_pointer_tail ]; 
+      entailer.
+  }
+  { (* l1 is not empty *)
+    destruct l1; [ simpl list_1n_rep at 1; Intros; contradiction | ].
+    forward.
+    forward.
+    pose proof (list_cons_app l1 z).
+    destruct H3 as [l3 [a H3]].
+    destruct H3 as [H3 [H4 H5]].
+    rewrite H3.
+    sep_apply list_1n_split.
+    Intros head1' tail1'.
+    simpl list_1n_rep.
+    Intros tail1_prev.
+    subst tail1. subst tail1_prev.
+    unfold node_rep at 1.
+    forward.                            (* l1->tail->next = l2->head; *)
+    forward.
+    forward.                            (* l1->tail = l2->tail; *)
+    forward.
+    forward.
+    forward.                            (* l1->size += l2->size; *)
+    forward_call (p2, sizeof t_struct_list); [solve_free | ].
+                                        (* freeN(l, sizeof (struct list)); *)
+    entailer.
+    unfold_list_rep.
+    Exists head1 tail2.
+    rewrite <- H3.
+    rewrite Z_length_plus.
+    entailer!.
+    rewrite H3 at 2.
+    remember (list_prefix (z :: l1) (Datatypes.length l1)) as l3.
+    pose proof (list_1n_merge l3 (a :: l2) head1 tail1' 
+      head1' tail2 nullval nullval).
+    rewrite <- app_assoc.
+    simpl.
+    eapply derives_trans; [ | apply H10 ].
+    simpl list_1n_rep.
+    Exists head2.
+    unfold node_rep.
+    entailer!.
+  }
+  { (* l1 is empty *)
+    subst tail1.
+    destruct l1.
+    2: {
+      sep_apply list_tail_nullval.
+      Intros.
+    }
+    simpl list_1n_rep at 1.
+    forward.
+    forward.                            (* l1->head = l2->head; *)
+    forward.
+    forward.                            (* l1->tail = l2->tail; *)
+    forward.
+    forward.
+    forward.                            (* l1->size += l2->size; *)
+    forward_call (p2, sizeof t_struct_list); [solve_free | ].
+                                        (* freeN(l, sizeof (struct list)); *)
+    entailer!.
+    simpl.
+    unfold_list_rep.
+    Exists head2 tail2.
+    entailer!.
+  }
+Qed.
